<?xml version="1.0"?>


<!DOCTYPE rdf:RDF [
    <!ENTITY dcterms "http://purl.org/dc/terms/" >
    <!ENTITY lemon "http://lemon-model.net/lemon#" >
    <!ENTITY owl "http://www.w3.org/2002/07/owl#" >
    <!ENTITY dbnary "http://kaiko.getalp.org/dbnary#" >
    <!ENTITY xsd "http://www.w3.org/2001/XMLSchema#" >
    <!ENTITY rdfs "http://www.w3.org/2000/01/rdf-schema#" >
    <!ENTITY rdf "http://www.w3.org/1999/02/22-rdf-syntax-ns#" >
]>


<rdf:RDF xmlns="http://kaiko.getalp.org/dbnary#"
     xml:base="http://kaiko.getalp.org/dbnary"
     xmlns:rdfs="http://www.w3.org/2000/01/rdf-schema#"
     xmlns:owl="http://www.w3.org/2002/07/owl#"
     xmlns:xsd="http://www.w3.org/2001/XMLSchema#"
     xmlns:rdf="http://www.w3.org/1999/02/22-rdf-syntax-ns#"
     xmlns:dbnary="http://kaiko.getalp.org/dbnary#"
     xmlns:lemon="http://lemon-model.net/lemon#"
     xmlns:dcterms="http://purl.org/dc/terms/">
    <owl:Ontology rdf:about="http://kaiko.getalp.org/dbnary">
        <rdfs:label>dbnary</rdfs:label>
        <rdfs:seeAlso>http://kaiko.getalp.org/about-dbnary/</rdfs:seeAlso>
        <rdfs:comment xml:lang="en">DBnary: A lexicon model designed to allow the representation of lexical data extracted from wiktionary language editions (http://www.wiktionary.org/). The dbnary model extends the lemon model (http://lemon-model.net/lemon).</rdfs:comment>
        <owl:imports rdf:resource="http://lemon-model.net/lemon"/>
    </owl:Ontology>
    


    <!-- 
    ///////////////////////////////////////////////////////////////////////////////////////
    //
    // Annotation properties
    //
    ///////////////////////////////////////////////////////////////////////////////////////
     -->

    


    <!-- http://kaiko.getalp.org/dbnary#exampleSource -->

    <owl:AnnotationProperty rdf:about="&dbnary;exampleSource">
        <rdfs:domain rdf:resource="&lemon;UsageExample"/>
    </owl:AnnotationProperty>
    


    <!-- 
    ///////////////////////////////////////////////////////////////////////////////////////
    //
    // Object Properties
    //
    ///////////////////////////////////////////////////////////////////////////////////////
     -->

    


    <!-- http://kaiko.getalp.org/dbnary#meronym -->

    <owl:ObjectProperty rdf:about="&dbnary;meronym">
        <rdfs:comment xml:lang="en">An underspecified meronymy relation between LexicalEntities (Lexical entries or Lexical Senses). This relation is used to encode an information available in a lexicon when the linked Lexical Senses are not known. When both source and target of the relation are Lexical Senses, one should use the corresponding LEMON relation. </rdfs:comment>
        <rdfs:subPropertyOf rdf:resource="&dbnary;topNymProperty"/>
    </owl:ObjectProperty>




<!-- http://kaiko.getalp.org/dbnary#antonym -->

    <owl:ObjectProperty rdf:about="&dbnary;antonym">
        <rdfs:comment xml:lang="en">An underspecified antonymy relation between LexicalEntities (Lexical entries or Lexical Senses). This relation is used to encode an information available in a lexicon when the linked Lexical Senses are not known. When both source and target of the relation are Lexical Senses, one should use the corresponding LEMON relation. </rdfs:comment>
        <rdfs:subPropertyOf rdf:resource="&dbnary;topNymProperty"/>
    </owl:ObjectProperty>
    


    <!-- http://kaiko.getalp.org/dbnary#approximateSynonym -->

    <owl:ObjectProperty rdf:about="&dbnary;approximateSynonym">
        <rdfs:comment xml:lang="en">An underspecified approximate synonymy relation between LexicalEntities (Lexical entries or Lexical Senses). This relation is used to encode an information available in a lexicon when the linked Lexical Senses are not known. When both source and target of the relation are Lexical Senses, one should use the corresponding LEMON relation. </rdfs:comment>
        <rdfs:subPropertyOf rdf:resource="&dbnary;topNymProperty"/>
    </owl:ObjectProperty>
    

    <!-- http://kaiko.getalp.org/dbnary#holonym -->

    <owl:ObjectProperty rdf:about="&dbnary;holonym">
        <rdfs:comment xml:lang="en">An underspecified holonymy relation between LexicalEntities (Lexical entries or Lexical Senses). This relation is used to encode an information available in a lexicon when the linked Lexical Senses are not known. When both source and target of the relation are Lexical Senses, one should use the corresponding LEMON relation. </rdfs:comment>
        <rdfs:subPropertyOf rdf:resource="&dbnary;topNymProperty"/>
    </owl:ObjectProperty>



    <!-- http://kaiko.getalp.org/dbnary#etymologicallyRelatedTo -->

    <owl:ObjectProperty rdf:about="&dbnary;etymologicallyRelatedTo">
	<rdfs:comment xml:lang="en">An underspecified etymological relationship betwen two LexicalEntries. </rdfs:comment>
        <rdfs:domain rdf:resource="&dbnary;LexicalEntry"/>
	<rdfs:range rdf:resource="&dbnary;LexicalEntry"/>
    </owl:ObjectProperty>




    <!-- http://kaiko.getalp.org/dbnary#etymologicallyEquivalentTo -->

    <owl:ObjectProperty rdf:about="&dbnary;etymologicallyEquivalentTo">
        <rdfs:comment xml:lang="en">The target and the source LexicalEntries share the same etymological origin. </rdfs:comment>
        <rdfs:domain rdf:resource="&dbnary;LexicalEntry"/>
        <rdfs:range rdf:resource="&dbnary;LexicalEntry"/>
        <rdfs:subPropertyOf rdf:resource="&dbnary;etymologicallyRelatedTo"/>
    </owl:ObjectProperty>
    



    <!-- http://kaiko.getalp.org/dbnary#etymologicallyDerivesFrom -->

    <owl:ObjectProperty rdf:about="&dbnary;etymologicallyDerivesFrom">
        <rdfs:comment xml:lang="en">The target LexicalEntry etymologically derives from the source LexicalEntry. </rdfs:comment>
        <rdfs:domain rdf:resource="&dbnary;LexicalEntry"/>
        <rdfs:range rdf:resource="&dbnary;LexicalEntry"/>
      	<rdfs:subPropertyOf rdf:resource="&dbnary;etymologicallyRelatedTo"/>
    </owl:ObjectProperty>


<!-- http://kaiko.getalp.org/dbnary#descendsFrom -->

    <owl:ObjectProperty rdf:about="&dbnary;descendsFrom">
        <rdfs:comment xml:lang="en">The target LexicalEntry is a descendant of the source LexicalEntry. </rdfs:comment>
	<rdfs:domain rdf:resource="&dbnary;LexicalEntry"/>
	<rdfs:range rdf:resource="&dbnary;LexicalEntry"/>
	<rdfs:subPropertyOf rdf:resource="&dbnary;etymologicallyRelatedTo"/>
    </owl:ObjectProperty>



<!-- http://kaiko.getalp.org/dbnary#derivesFrom -->

    <owl:ObjectProperty rdf:about="&dbnary;derivesFrom">
	<rdfs:comment xml:lang="en">The target LexicalEntry is a term derived from the source LexicalEntry. E.g.:eng:link_up derivesFrom eng:link_ety_1. </rdfs:comment>
	<rdfs:domain rdf:resource="&dbnary;LexicalEntry"/>
	<rdfs:range rdf:resource="&dbnary;LexicalEntry"/>
	<rdfs:subPropertyOf rdf:resource="&dbnary;etymologicallyRelatedTo"/>
    </owl:ObjectProperty>




    <!-- http://kaiko.getalp.org/dbnary#hypernym -->

    <owl:ObjectProperty rdf:about="&dbnary;hypernym">
        <rdfs:comment xml:lang="en">An underspecified hypernymy relation between LexicalEntities (Lexical entries or Lexical Senses). This relation is used to encode an information available in a lexicon when the linked Lexical Senses are not known. When both source and target of the relation are Lexical Senses, one should use the corresponding LEMON relation. </rdfs:comment>
        <rdfs:subPropertyOf rdf:resource="&dbnary;topNymProperty"/>
    </owl:ObjectProperty>
    


    <!-- http://kaiko.getalp.org/dbnary#hyponym -->

    <owl:ObjectProperty rdf:about="&dbnary;hyponym">
        <rdfs:comment xml:lang="en">An underspecified hyponymy relation between LexicalEntities (Lexical entries or Lexical Senses). This relation is used to encode an information available in a lexicon when the linked Lexical Senses are not known. When both source and target of the relation are Lexical Senses, one should use the corresponding LEMON relation. </rdfs:comment>
        <rdfs:subPropertyOf rdf:resource="&dbnary;topNymProperty"/>
    </owl:ObjectProperty>
    


    <!-- http://kaiko.getalp.org/dbnary#isTranslationOf -->

    <owl:ObjectProperty rdf:about="&dbnary;isTranslationOf">
        <rdfs:comment xml:lang="en">links the translation information to the Lexical Entity it belongs to.</rdfs:comment>
        <rdfs:range rdf:resource="&dbnary;LexicalEntity"/>
        <rdfs:domain rdf:resource="&dbnary;Translation"/>
    </owl:ObjectProperty>
    


    <!-- http://kaiko.getalp.org/dbnary#meronym -->

    <owl:ObjectProperty rdf:about="&dbnary;meronym">
        <rdfs:comment xml:lang="en">An underspecified meronymy relation between LexicalEntities (Lexical entries or Lexical Senses). This relation is used to encode an information available in a lexicon when the linked Lexical Senses are not known. When both source and target of the relation are Lexical Senses, one should use the corresponding LEMON relation. </rdfs:comment>
        <rdfs:subPropertyOf rdf:resource="&dbnary;topNymProperty"/>
    </owl:ObjectProperty>
    


    <!-- http://kaiko.getalp.org/dbnary#refersTo -->

    <owl:ObjectProperty rdf:about="&dbnary;refersTo">
        <rdfs:comment xml:lang="en">links a vocable to any lexical entry that share the same written form. </rdfs:comment>
        <rdfs:domain rdf:resource="&dbnary;Vocable"/>
        <rdfs:range rdf:resource="&lemon;LexicalEntry"/>
    </owl:ObjectProperty>
    


    <!-- http://kaiko.getalp.org/dbnary#synonym -->

    <owl:ObjectProperty rdf:about="&dbnary;synonym">
        <rdfs:comment xml:lang="en">An underspecified synonymy relation between LexicalEntities (Lexical entries or Lexical Senses). This relation is used to encode an information available in a lexicon when the linked Lexical Senses are not known. When both source and target of the relation are Lexical Senses, one should use the corresponding LEMON relation. </rdfs:comment>
        <rdfs:subPropertyOf rdf:resource="&dbnary;topNymProperty"/>
    </owl:ObjectProperty>
    


    <!-- http://kaiko.getalp.org/dbnary#targetLanguage -->

    <owl:ObjectProperty rdf:about="&dbnary;targetLanguage">
        <rdf:type rdf:resource="&owl;FunctionalProperty"/>
        <rdfs:comment xml:lang="en">The target language of a given translation, defined as a Linguistic System.</rdfs:comment>
        <rdfs:domain rdf:resource="&dbnary;Translation"/>
        <rdfs:range rdf:resource="&dcterms;LinguisticSystem"/>
    </owl:ObjectProperty>
    


    <!-- http://kaiko.getalp.org/dbnary#topNymProperty -->

    <owl:ObjectProperty rdf:about="&dbnary;topNymProperty">
        <rdfs:comment xml:lang="en">An underspecified lexico semantic relation between LexicalEntities (Lexical entry OR Lexical Sense). This relation is used to encode an information available in a lexicon when the linked Lexical Senses are not known. When both source and target of the relation are Lexical Senses, one should use the corresponding LEMON relation. </rdfs:comment>
        <rdfs:range rdf:resource="&dbnary;LexicalEntity"/>
        <rdfs:domain rdf:resource="&dbnary;LexicalEntity"/>
    </owl:ObjectProperty>
    


    <!-- http://kaiko.getalp.org/dbnary#troponym -->

    <owl:ObjectProperty rdf:about="&dbnary;troponym">
        <rdfs:comment xml:lang="en">A verb that indicates more precisely the manner of doing something by replacing a verb of a more generalized meaning. E.g.: &quot;Stroll&quot; is a troponym of &quot;walk&quot;, since it involves a slow and relaxed sort of walking.</rdfs:comment>
        <rdfs:subPropertyOf rdf:resource="&dbnary;topNymProperty"/>
    </owl:ObjectProperty>
    


    <!-- 
    ///////////////////////////////////////////////////////////////////////////////////////
    //
    // Data properties
    //
    ///////////////////////////////////////////////////////////////////////////////////////
     -->

    


    <!-- http://kaiko.getalp.org/dbnary#exampleSource -->

    <owl:DatatypeProperty rdf:about="&dbnary;exampleSource"/>
    


    <!-- http://kaiko.getalp.org/dbnary#gloss -->

    <owl:DatatypeProperty rdf:about="&dbnary;gloss">
        <rdfs:comment xml:lang="en">A textual gloss that may be used to disambiguate the translation&apos;s source sense. </rdfs:comment>
        <rdfs:domain rdf:resource="&dbnary;Translation"/>
        <rdfs:range rdf:resource="&xsd;string"/>
    </owl:DatatypeProperty>
    


    <!-- http://kaiko.getalp.org/dbnary#note -->

    <owl:DatatypeProperty rdf:about="&dbnary;note">
        <rdfs:comment xml:lang="en">Textual note that may be used to add information to a LemonElement when no standard vocabularies exists to explicit it.</rdfs:comment>
        <rdfs:domain rdf:resource="&lemon;LemonElement"/>
        <rdfs:range rdf:resource="&xsd;string"/>
    </owl:DatatypeProperty>
    


    <!-- http://kaiko.getalp.org/dbnary#partOfSpeech -->

    <owl:DatatypeProperty rdf:about="&dbnary;partOfSpeech">
        <rdfs:comment xml:lang="en">The original part of speech as it was defined in the Wiktionary page. This property takes a String litteral as object.</rdfs:comment>
        <rdfs:domain rdf:resource="&lemon;LexicalEntry"/>
        <rdfs:range rdf:resource="&xsd;string"/>
    </owl:DatatypeProperty>
    


    <!-- http://kaiko.getalp.org/dbnary#senseNumber -->

    <owl:DatatypeProperty rdf:about="&dbnary;senseNumber">
        <rdfs:comment xml:lang="en">The number of the lexical Sense in the Lexical Entry, as given by Wiktionary. This property takes a String literal as an object.</rdfs:comment>
        <rdfs:domain rdf:resource="&lemon;LexicalSense"/>
    </owl:DatatypeProperty>
    


    <!-- http://kaiko.getalp.org/dbnary#targetLanguageCode -->

    <owl:DatatypeProperty rdf:about="&dbnary;targetLanguageCode">
        <rdf:type rdf:resource="&owl;FunctionalProperty"/>
        <rdfs:comment xml:lang="en">The target language of a given translation. This may be used when the dbnary:targetLanguage object property can not be used.</rdfs:comment>
        <rdfs:domain rdf:resource="&dbnary;Translation"/>
        <rdfs:range rdf:resource="&xsd;string"/>
    </owl:DatatypeProperty>
    


    <!-- http://kaiko.getalp.org/dbnary#usage -->

    <owl:DatatypeProperty rdf:about="&dbnary;usage">
        <rdfs:comment xml:lang="en">Usage note that is used to further annotate the target of the translation.</rdfs:comment>
        <rdfs:domain rdf:resource="&dbnary;Translation"/>
        <rdfs:range rdf:resource="&xsd;string"/>
    </owl:DatatypeProperty>
    


    <!-- http://kaiko.getalp.org/dbnary#writtenForm -->

    <owl:DatatypeProperty rdf:about="&dbnary;writtenForm">
        <rdfs:comment xml:lang="en">The written form of a translation equivalent.</rdfs:comment>
        <rdfs:domain rdf:resource="&dbnary;Translation"/>
        <rdfs:range rdf:resource="&xsd;string"/>
    </owl:DatatypeProperty>
    


    <!-- 
    ///////////////////////////////////////////////////////////////////////////////////////
    //
    // Classes
    //
    ///////////////////////////////////////////////////////////////////////////////////////
     -->

    


    <!-- http://kaiko.getalp.org/dbnary#LexicalEntity -->

    <owl:Class rdf:about="&dbnary;LexicalEntity">
        <rdfs:subClassOf rdf:resource="&lemon;LemonElement"/>
        <owl:disjointUnionOf rdf:parseType="Collection">
            <rdf:Description rdf:about="&lemon;LexicalEntry"/>
            <rdf:Description rdf:about="&lemon;LexicalSense"/>
        </owl:disjointUnionOf>
    </owl:Class>
    


    <!-- http://kaiko.getalp.org/dbnary#Translation -->

    <owl:Class rdf:about="&dbnary;Translation">
        <rdfs:subClassOf rdf:resource="&owl;Thing"/>
        <rdfs:comment xml:lang="en">Describe translation information for a Lexical Entry or a Lexical Sense.</rdfs:comment>
    </owl:Class>
    


    <!-- http://kaiko.getalp.org/dbnary#Vocable -->

    <owl:Class rdf:about="&dbnary;Vocable">
        <rdfs:subClassOf rdf:resource="&lemon;LexicalEntry"/>
        <rdfs:comment xml:lang="en">A Vocable corresponds to a set of Lexical Entries that usually share the same written form but that do not necessarily share the same Part Of Speech. E.g. cat_n and cat_v are distinct lexical entries while the vocable &quot;cat&quot; refers to both of them.</rdfs:comment>
    </owl:Class>
    

    <owl:Class rdf:about="&dbnary;EtymologyEntry">
        <rdfs:subClassOf rdf:resource="&lemon;LexicalEntry"/>
        <rdfs:comment xml:lang="en">An EtymologyEntry corresponds to a set of Lexical Entries that share the same etymology but that do not necessarily share the same Part Of Speech. E.g. eng:link_n_1 and eng:link_v_1 are distinct lexical entries and the etymology entry link_ety_1 refers to both of them because link_n_1 and link_v_1 share the same etymology from Old English ang:linke.</rdfs:comment>
    </owl:Class>

    <!-- http://lemon-model.net/lemon#LemonElement -->

    <owl:Class rdf:about="&lemon;LemonElement"/>
    


    <!-- http://lemon-model.net/lemon#LexicalEntry -->

    <owl:Class rdf:about="&lemon;LexicalEntry"/>
    


    <!-- http://lemon-model.net/lemon#LexicalSense -->

    <owl:Class rdf:about="&lemon;LexicalSense"/>
    


    <!-- http://purl.org/dc/terms/LinguisticSystem -->

    <owl:Class rdf:about="&dcterms;LinguisticSystem"/>
</rdf:RDF>



<!-- Generated by the OWL API (version 3.5.0) http://owlapi.sourceforge.net -->

 
